Tables/Error.lean
@@ -8,9 +8,12 @@ public section
 namespace Tables
 
 inductive Error where
+  | columnNotFound (name : String)
   | duplicateColumnName (name : String)
   | mismatchedRowCount (expected : Nat) (actual : Nat)
   | mismatchedSchema (expected : Schema) (actual : Schema)
+  | overlappingColumnName (name : String)
+  | schemaNotWellFormed
 deriving Repr, DecidableEq
 
 end Tables
